\documentclass[a4paper]{article}

\usepackage[english]{babel}
\usepackage[utf8x]{inputenc}
\usepackage{amsmath}
\usepackage{graphicx}
\usepackage{cleveref}
\usepackage{mathtools}
\usepackage{fancyhdr}
\numberwithin{equation}{subsection}
\usepackage[english]{babel}
 
\newtheorem{theorem}{Theorem}[section]
\newtheorem{corollary}{Corollary}[theorem]
\newtheorem{lemma}[theorem]{Lemma}
\newtheorem{definition}{Definition}[section]

\fancyhf{}
\fancyhead[LE,RO]{\thepage}
\fancyhead[CE]{\Author}
\fancyhead[CO]{\Title}
\renewcommand\headrulewidth{0pt}
\pagestyle{fancy}

\author{Emil Kerimov}
%\title{Basic Trig Functions}

\makeatletter
\let\Title\@author

\begin{document}
\section{Geometric Series}\label{Geometric Series}

Prove that:

$$\sum\limits_{i=1}^{n} a\cdot r^{i-1} =  \frac{a\cdot(1-r^{n+1})}{1-r}$$

Proof:

Define $S_n$ such that:

$$S_{n} = a + ar + ar^2 + ... + ar^{n-1}+ar^n$$
Note that $$r\cdot S_{n} = ar + ar^2 + ... + ar^{n-1} + ar^n + ar^{n+1}$$
Such that $$S_{n}-r\cdot S_{n} = a-ar^{n+1}$$
$$=>
S_{n} = \frac{a\cdot(1-r^{n+1})}{1-r}
$$


If $|r|<1$:

Then 
$$\sum\limits_{i=1}^{\infty} a\cdot r^{i-1}
= \lim_{n \to +\infty}\frac{a\cdot(1-r^{n+1})}{1-r}
= \frac{a}{1-r}
$$

Note that by taking derivatives of both sides and a bit of reindexing:

$$\sum\limits_{i=0}^{\infty} \frac{d}{dr}a\cdot r^{i}
=\sum\limits_{i=0}^{\infty} i\cdot a\cdot r^{i-1}
=0+\sum\limits_{i=1}^{\infty} i\cdot a\cdot r^{i-1}
= \frac{a}{(1-r)^2}
$$

$$=>
\sum\limits_{i=1}^{\infty} i\cdot r^{i}
= \frac{r}{(1-r)^2} \mbox{ when } |r|<1
$$
\end{document}