\documentclass[a4paper]{article}

\usepackage[english]{babel}
\usepackage[utf8x]{inputenc}
\usepackage{amsmath}
\usepackage{graphicx}
\usepackage{cleveref}
\usepackage{mathtools}
\usepackage{fancyhdr}
\numberwithin{equation}{subsection}
\usepackage[english]{babel}
 
\newtheorem{theorem}{Theorem}[section]
\newtheorem{corollary}{Corollary}[theorem]
\newtheorem{lemma}[theorem]{Lemma}
\newtheorem{definition}{Definition}[section]

\fancyhf{}
\fancyhead[LE,RO]{\thepage}
\fancyhead[CE]{\Author}
\fancyhead[CO]{\Title}
\renewcommand\headrulewidth{0pt}
\pagestyle{fancy}

\author{Emil Kerimov}
%\title{Basic Trig Functions}

\makeatletter
\let\Title\@author


\begin{document}


\section{Integral Representation of Zeta(2)}\label{Integral Representation of Zeta(2)} 

$$
\int_{0}^{\infty}\frac{t}{e^{\alpha t}-1}dt
=\int_{0}^{\infty}\frac{te^{-\alpha t}}{1-e^{-\alpha t}}dt 
= \int_{0}^{\infty} t\sum\limits_{n=1}^{\infty} e^{-n\alpha t}dt
$$

By the Dominant Convergence Theorem: (Include Reference)

$$ \int_{0}^{\infty} t\sum\limits_{n=1}^{\infty} e^{-n\alpha t} dt
=\sum\limits_{n=1}^{\infty} \int_{0}^{\infty}  te^{-n\alpha t}dt$$

Using  $n\cdot \alpha \cdot t = x  \rightarrow n\cdot \alpha \cdot dt = dx$ 
$$
\sum\limits_{n=1}^{\infty} \int_{0}^{\infty}  \frac{x}{n\alpha}e^{-x}\frac{dx}{n\alpha}
=\sum\limits_{n=1}^{\infty} \frac{1}{n^2 \alpha^2 }\int_{0}^{\infty}  xe^{-x}dx
=\frac{1}{\alpha^2}\sum\limits_{n=1}^{\infty} \frac{1}{n^2}\Gamma(2)
$$

Recall $\Gamma(2) = 1! = 1$ (Include Reference)

$$\frac{1}{\alpha^2}\sum\limits_{n=1}^{\infty} \frac{1}{n^2}\Gamma(2)
=\frac{1}{\alpha^2}\sum\limits_{n=1}^{\infty} \frac{1}{n^2}
= \frac{1}{\alpha^2} \zeta(2)
$$

Recall $\zeta(2) = \frac{\pi^2}{6}$ (Include Reference)

$$
=>   \int_{0}^{\infty}\frac{t}{e^{\alpha t}-1}dt
=\frac{\pi^2}{6\alpha^2}
$$

\end{document}