\documentclass[a4paper]{article}

\usepackage[english]{babel}
\usepackage[utf8x]{inputenc}
\usepackage{amsmath}
\usepackage{graphicx}
\usepackage[colorinlistoftodos]{todonotes}
\usepackage{mathtools}

\title{Technique Recursive sum of powers}
\author{Emil Kerimov}
\date{\today}
\begin{document}
\maketitle

\section{Technique Recursive sum of powers}
\label{Recursive sum of powers}

To solve for $\sum\limits_{i=1}^{n} i^{p}$ consider $\sum\limits_{i=1}^{n} {(1+i)^{p+1} - i^{p+1}} = (1+n)^{p+1} - 1$

\subsection{Sum of Squares}

Let p=2

$$\sum\limits_{i=1}^{n} (1+i)^3 - i^3 = \sum\limits_{i=1}^{n} 1+3i+3i^2 +i^3 - i^3 = \sum\limits_{i=1}^{n} 1+3i+3i^2$$

and 

$$\sum\limits_{i=1}^{n} (1+i)^3 - i^3 = (n+1)^3 - 1$$

Hence

$$\sum\limits_{i=1}^{n} 1+ 3\sum\limits_{i=1}^{n}i+3\sum\limits_{i=1}^{n}i^2 =(n+1)^3 - 1$$

$$n+3\frac{n(n-1)}{2}+3\sum\limits_{i=1}^{n}i^2 =(n+1)^3 - 1$$


$$3\sum\limits_{i=1}^{n}i^2 = n^3 + 3n^2 + 3n + 1 - n - 3\frac{n(n-1)}{2}$$


$$3\sum\limits_{i=1}^{n}i^2 = n(n+1)(n+\frac{1}{2})$$


$$
\boxed{
\sum\limits_{i=1}^{n}i^2 = \frac{n}{3} \cdot (n+1) \cdot (n+\frac{1}{2})
}
$$

\subsection{Sum of Cubes}

Let p=3

$$\sum\limits_{i=1}^{n} (1+i)^4 - i^4 = \sum\limits_{i=1}^{n} 1+4i+6i^2 + 4i^3 +i^4 - i^4 = \sum\limits_{i=1}^{n} 1+4i+6i^2 + 4i^3$$

and 

$$\sum\limits_{i=1}^{n} (1+i)^4 - i^4 = (n+1)^4 - 1$$

Hence

$$\sum\limits_{i=1}^{n} 1+ 4\sum\limits_{i=1}^{n}i + 6\sum\limits_{i=1}^{n}i^2
+ 4\sum\limits_{i=1}^{n}i^3 =(n+1)^4 - 1$$

$$n+4\frac{n(n-1)}{2}+6 \frac{n}{3} \cdot (n+1) \cdot (n+\frac{1}{2}) + 4\sum\limits_{i=1}^{n}i^3 =(n+1)^4 - 1$$


$$4\sum\limits_{i=1}^{n}i^3 = n^4 + 4n^3 + 6n^2 + 4n - n - 2n(n-1) - n\cdot (n+1) \cdot (2n+1)$$

Simplifying

$$4\sum\limits_{i=1}^{n}i^3 = n^4 + 2n^3 + n^2 $$

$$4\sum\limits_{i=1}^{n}i^3 = n^2 (n^2 + 2n + 1) = n^2(n+1)^2$$

$$
\boxed{
\sum\limits_{i=1}^{n}i^3 = \Big( \frac{n(n+1)}{2} \Big)^2
}
$$

\end{document}