\documentclass[a4paper]{article}

\usepackage[english]{babel}
\usepackage[utf8x]{inputenc}
\usepackage{amsmath}
\usepackage{graphicx}
\usepackage[colorinlistoftodos]{todonotes}
\usepackage{mathtools}
\usepackage{amssymb}

\title{Bernoulli Numbers}
\author{Emil Kerimov}
\date{\today}
\begin{document}
    \maketitle

    \newtheorem{theorem}{Theorem}[section]
    \newtheorem{corollary}{Corollary}[theorem]
    \newtheorem{lemma}[theorem]{Lemma}
    \newtheorem{definition}{Definition}[section]


    \section{Bernoulli Numbers}\label{sec:bernoulli-numbers}
    Examining the Taylor expansion of $\frac{x}{e^x -1}$, this will be required for the evaluation of the even integer values of $\zeta.$

    \begin{definition}
        \label{bernoulli def}
        The Bernoulli numbers $B_n$ are defined as the coefficients of the Taylor expansion of the following function
        \[\boxed{
            \frac{x}{e^x -1} = \sum_{n=0}^{\infty} \frac{B_n}{n!} x^n
        }
        \]
    \end{definition}

    \begin{theorem}
        \begin{equation}
            \label{eq:bernoulli-generating}
            \sum_{k}^{n} \binom{n+1}{k} B_k = 0  \quad \forall n > 0, \text{ with } B_0 = 1
        \end{equation}

        Proof
        \begin{gather*}
            \intertext{Starting from definition~\ref{bernoulli def}}
            \frac{x}{e^x -1} = \sum_{n=0}^{\infty} \frac{B_n}{n!} x^n
            \\
            \intertext{Using the Taylor expansion of $e^x$}
            \frac{x}{\sum_{k=1}^{\infty} \frac{x^k}{k!}} = \sum_{n=0}^{\infty} \frac{B_n}{n!} x^n
            \\
            \intertext{Rearranging}
            x = \sum_{k=1}^{\infty} \frac{x^k}{k!} \sum_{n=0}^{\infty} \frac{B_n}{n!} x^n
            \\
            1 = \sum_{k=1}^{\infty} \frac{x^{k-1}}{k!} \sum_{n=0}^{\infty} \frac{B_n}{n!} x
            \\
            \intertext{Adjusting the indices}
            1 = \sum_{k=0}^{\infty} \frac{x^{k}}{(k+1)!} \sum_{n=0}^{\infty} \frac{B_n}{n!} x^n
            \\
            \intertext{Using Cauchy's product formula for infinite sums \footnotemark}
            1 = \sum_{n=0}^{\infty}
            \underbrace{\sum_{k=0}^{n}
                \underbrace{\Big(\frac{B_k}{k!} x^k \Big)}_{a_k}
                \underbrace{\Big(\frac{x^{n-k}}{(n-k+1)!} \Big)}_{b_{n-k}}}_{c_n}
            \\
            \intertext{Simplifying}
            1 = \sum_{n=0}^{\infty}
            \frac{1}{(n+1)!}
            \sum_{k=0}^{n}
            \binom{n+1}{k}
            B_k x^k x^{n-k}
            \\
            1 = \sum_{n=0}^{\infty}
            \frac{x^n}{(n+1)!}
            \sum_{k=0}^{n}  \binom{n+1}{k} B_k
            \intertext{Comparing coefficients of powers of $x$ of both sides we get}
            n=0, \quad  1 =  B_0
            \\
            n \not =0, \quad 0= \sum_{k=0}^{n}  \binom{n+1}{k} B_k
        \end{gather*}
    \end{theorem}

    \footnotetext{$\Big\left( \sum_{n=0}^{\infty} a_n \Big\right) \Big\left( \sum_{n=0}^{\infty} b_n \Big\right) = \sum_{n=0}^{\infty} c_n $ where $c_n = \sum_{k=0}^{n} a_k b_{n-k}$. See proof: TODO ADD}

    \subsection{First few Bernoulli numbers}\label{subsec:first-few-bernoulli-numbers}
    Using equation~\ref{eq:bernoulli-generating} with $n=1$ implies $ \binom{2}{0} B_0 + \binom{2}{1} B_1 = 0 = 1 + 2 B_1 $ which implies
    \begin{equation}
        B_1 = -\frac{1}{2}\label{eq:equation}
    \end{equation}

    Using equation~\ref{eq:bernoulli-generating} with $n=2$ implies $ \binom{3}{0} B_0 + \binom{3}{1} B_1 + \binom{3}{2} B_2 = 0 = 1 - \frac{3}{2} + 3 B_2 $ which implies
    \begin{equation}
        B_2 = \frac{1}{6}\label{eq:equation2}
    \end{equation}

    Similarly when we apply this equation for increasing values of n
    \begin{equation}
        B_3 = 0, B_4 = -\frac{1}{30}, B_5 = 0, B_6 = \frac{1}{42}, \dots \label{eq:equation3}
    \end{equation}


    \begin{theorem}
        In fact we can show that all odd Bernoulli numbers after n=1 are 0
        \begin{equation}
            \label{eq:odd-bernoulli} B_n = 0  \quad \forall \text{ odd }n > 1
        \end{equation}

        Proof
        \begin{gather*}
            \intertext{Starting from definition~\ref{bernoulli def}}
            \frac{x}{e^x -1} = \sum_{n=0}^{\infty} \frac{B_n}{n!} x^n
            \\
            \intertext{Removing the first two terms of the sum}
            \frac{x}{e^x -1} = B_0 + B_1 x + \sum_{n=2}^{\infty} \frac{B_n}{n!} x^n\\
            \intertext{Rearranging}
            \frac{x}{e^x -1}  - 1 + \frac{x}{2}= \sum_{n=2}^{\infty} \frac{B_n}{n!} x^n
            \\
            \frac{x + xe^x}{2e^x -2}  - 1 = \sum_{n=2}^{\infty} \frac{B_n}{n!} x^n
            \\
            \intertext{If we can show that the RHS is an even function then we have established the proof}
            y(x) = \frac{x + xe^x}{2e^x -2}  - 1
            \\
            y(-x) = \frac{-x + -xe^{-x}}{2e^{-x} -2}  - 1
            \\
            \intertext{Simplifying}
            y(-x) = \frac{-x -xe^{-x}}{2e^{-x} -2} \cdot \frac{e^x}{e^x}  - 1
            \\
            y(-x) = \frac{-xe^x -x}{2 -2e^x}  - 1
            \\
            y(-x) = \frac{x+xe^x}{2e^x - 2}  - 1
            \\
            y(-x) = y(x)
            \\
            B_n = 0  \quad \forall \text{ odd }n > 1
        \end{gather*}
    \end{theorem}

    \pagebreak


    \section{Bernoulli Polynomials}\label{sec:bernoulli-polynomials}
    \begin{definition}
        \label{bernoulli poly def}
        The Bernoulli polynomials $B_n(x)$ are defined as
        \[\boxed{
            B_{n}(x) = \sum_{k=0}^{n} {n \choose k} B_k x^{n-k}
        }\]
    \end{definition}

    \subsection{Examples}\label{subsec:examples}
    \begin{align*}
        B_{0}(x) &= B_0 = 1
        \\
        B_{1}(x) &= B_0 x + B_1 = x - \frac{1}{2}
        \\
        B_{2}(x) &= B_0 x^2 + {2 \choose 1} B_1 x + B_2 = x^2 - x +  \frac{1}{6}
        \\
        B_{3}(x) &= B_0 x^3 + {3 \choose 1} B_1 x^2 + {3 \choose 2} B_2 x + B_3 = x^3 - \frac{3}{2} x^2 +  \frac{1}{2} x
    \end{align*}

    Note that $B_n(x)$ is a polynomial of degree $n$.

    \subsection{Useful Properties}\label{subsec:useful-properties}
    \begin{theorem}
        $B_n(0)$
        \begin{equation}
            \boxed{B_n(0) = B_n}\label{eq:equation4}
        \end{equation}
        Proof
        \begin{gather*}
            B_n(x) = \sum_{k=0}^{n} {n \choose k} B_k x^{n-k}
            \\
            B_n(x) = \sum_{k=0}^{n-1} {n \choose k} B_k x^{n-k} + B_n
            \\
            B_n(0) = \sum_{k=0}^{n-1} {n \choose k} B_k \cdot 0 + B_n = B_n
        \end{gather*}
    \end{theorem}

    \begin{theorem}
        $B_n(1)$  % todo format better using piecewise
        \begin{equation}
            \boxed{B_n(1) = B_n \quad n\neq 1
            \quad B_1(1) = -B_1}\label{eq:equation5}
        \end{equation}
        Proof
        \begin{gather*}
            B_n(x) = \sum_{k=0}^{n} {n \choose k} B_k x^{n-k}
            \\
            B_n(1) = \sum_{k=0}^{n} {n \choose k} B_k
            \intertext{Using equation~\ref{eq:bernoulli-generating}, $\sum_{k}^{n} \binom{n+1}{k} B_k = 0$}
            \sum_{k}^{n-1} \binom{n}{k} B_k = 0
            \intertext{Adding $B_n$ to both sides}
            \sum_{k}^{n} \binom{n}{k} B_k = B_n
        \end{gather*}
    \end{theorem}

    \begin{theorem}
        Derivative
        \begin{equation}
            \boxed{B^{'}_n(x) = n B_{n-1}(x)}\label{eq:equation6}
        \end{equation}
        Proof
        \begin{gather*}
            B_n(x) = \sum_{k=0}^{n} {n \choose k} B_k x^{n-k}
            \intertext{Taking derivatives of both sides}
            B^{'}_n(x) = \sum_{k=0}^{n-1} {n \choose k} B_k (n-k) x^{n-k-1}
            \\
            B^{'}_n(x) = \sum_{k=0}^{n-1} \frac{n! (n-k)}{k! (n-k)!} B_k x^{n-1-k}
            \\
            B^{'}_n(x) = \sum_{k=0}^{n-1} \frac{(n-1)! \cdot n}{k! (n-k-1)!} B_k x^{n-1-k}
            \\
            B^{'}_n(x) = n \sum_{k=0}^{n-1} {n-1 \choose k} B_k x^{n-1-k}
            \\
            B^{'}_n(x) = n B_{n-1}(x)
        \end{gather*}
    \end{theorem}

    \begin{theorem}
        Integral
        \begin{equation}
            \boxed{\int_{x=0}^{1} B_n(x) dx = 0}\label{eq:equation7}
        \end{equation}
        Proof
        \begin{gather*}
            \intertext{Starting from the derivative equation, using $m=n-1$}
            B^{'}_{m+1}(x) = (m+1) \cdot B_{m}(x)
            \intertext{Integrating both sides}
            \int_{x=0}^{1} B^{'}_{m+1}(x) = B_{m+1}(1) - B_{m+1}(0) = (m+1) \cdot  \int_{x=0}^{1} B_{m}(x)
            \intertext{Using the Bernoulli polynomial properties}
            B_{m+1}(1) - B_{m+1}(0) = B_{m+1} - B_{m+1} = 0
            \intertext{Therefore for $m \neq -1$}
            \int_{x=0}^{1} B_{m}(x) = 0
        \end{gather*}
    \end{theorem}

    \pagebreak


    \section{Euler-Maclaurin formula}\label{sec:euler-maclaurin-formula}

    Let $ \{ x \} = x - \lfloor{x}\rfloor $ then

    \begin{theorem}
        \begin{subequations}
            \label{Euler-Maclaurin formula}
            \begin{align}
                \sum_{k=1}^{n-1} f(k) &= \int_{x=1}^{n} f(x) dx -
                \sum_{k=1}^{m} \frac{B_k}{k!} \cdot \big( f^{(k-1)}(n) - f^{(k-1)}(1) \big) +
                R_{mn} \\
                R_{mn} &= \frac{(-1)^{m+1}}{m!} \cdot \int_{x=1}^{n} B_{m}(\{x\}) f^{(m)} (x) dx
            \end{align}
        \end{subequations}

        Proof
        \begin{gather*}
            \intertext{See the Darboux Formula paper for proof}
        \end{gather*}
    \end{theorem}

    \subsection{Stirling's Approximation}\label{subsec:stirling's-approximation}
    \begin{theorem}
%\begin{equation} 
%n! = \Big( \frac{n}{e} \Big)^{n} \sqrt{2 \pi n} \cdot e^{\sum_{k=2}^{m} \frac{B_k}{k \cdot (k-1)} \cdot \frac{1}{n^{k-1}} + O(\frac{1}{n^{m}})} 
%\end{equation}

        \begin{equation}
            n! = \Big( \frac{n}{e} \Big)^{n} \sqrt{2 \pi n} \cdot exp\Bigg(\sum_{k=1}^{\lfloor m/2 \rfloor} \frac{B_{2k}}{2k \cdot (2k-1)}  \frac{1}{n^{2k-1}} + O(\frac{1}{n^{m}})\Bigg)\label{eq:equation8}
        \end{equation}


        Proof
        \begin{gather*}
            \intertext{See the Gamma function paper for proof}
        \end{gather*}
    \end{theorem}

    \pagebreak


    \section{Connection to $\zeta(2n)$}\label{sec:connection-to-$zeta(2n)$}

    See the Zeta function document.

    \begin{theorem}
        We can express all even integer values of $\zeta$ using Bernoulli numbers
        \begin{equation}
            \label{eq:even-zeta}
            \zeta(2n) = (-1)^{n+1} \frac{(2\pi)^{2n} B_{2n}}{2 \cdot (2n)!}
        \end{equation}

        Proof:
        See the Zeta function document.
    \end{theorem}

    \subsection{The first few even integer values of $\zeta$}\label{subsec:the-first-few-even-integer-values-of-$zeta$}

    \begin{gather*}
        \zeta(2) = \frac{\pi^2}{6},
        \zeta(4) = \frac{\pi^4}{90},
        \zeta(6) = \frac{\pi^6}{945},
        \zeta(8) = \frac{\pi^8}{9450},
        \zeta(10) = \frac{\pi^{10}}{93555},
        \\
        \zeta(12) = \frac{691}{638512875} \pi^{12},
        \zeta(14) = \frac{2}{18243225} \pi^{14},
        \zeta(16) = \frac{3617}{325641566250} \pi^{16},
        \\
        \zeta(18) = \frac{43867}{38979295480125} \pi^{18},
        \zeta(20) = \frac{174611}{1531329465290625} \pi^{20},
        \zeta(22) = \frac{155366}{13447856940643125} \pi^{22},
        \\
        \zeta(24) = \frac{236364091}{201919571963756521875} \pi^{24},
        \dots
    \end{gather*}

    \pagebreak


\end{document}
