\documentclass[a4paper]{article}

\usepackage[english]{babel}
\usepackage[utf8x]{inputenc}
\usepackage{amsmath}
\usepackage{graphicx}
\usepackage{cleveref}
\usepackage{mathtools}
\usepackage{fancyhdr}
\numberwithin{equation}{subsection}
\usepackage[english]{babel}
 
\newtheorem{theorem}{Theorem}[section]
\newtheorem{corollary}{Corollary}[theorem]
\newtheorem{lemma}[theorem]{Lemma}
\newtheorem{definition}{Definition}[section]

\title{Gaussian Integral}
\author{Emil Kerimov}
\date{\today}
\begin{document}
\maketitle

\section{Gaussian Integral} 

\begin{theorem}
$$
\int_{-\infty}^{\infty}{e^{-ax^2}}dx = \sqrt{\frac{\pi}{a}}
$$
Proof

\begin{gather*}
\shortintertext{Defining $I$}
I = \int_{-\infty}^{\infty}{e^{-ax^2}}dx\\
\shortintertext{Squaring $I$}
I^2 = \int_{-\infty}^{\infty}{e^{-ax^2}}dx \cdot \int_{-\infty}^{\infty}{e^{-ay^2}}dy\\
\shortintertext{Combining the integrals}
I^2 = \int_{-\infty}^{\infty} \int_{-\infty}^{\infty}{e^{-ax^2 - ay^2}}dx dy\\
\shortintertext{Converting to Polar coordinates}
I^2 = \int_{0}^{2 \pi} \int_{0}^{\infty}{e^{-ar^2}}rdr d\theta\\
\shortintertext{Solving}
\begin{alignedat}{2}
I^2 &= \int_{0}^{2 \pi} \tfrac{-1}{2a} e^{-ar^2} \Big|_0^{\infty} d\theta \\
I^2 &= \int_{0}^{2 \pi} \tfrac{1}{2a} d\theta \\
I^2 &= 2 \pi \tfrac{1}{2a} \\
I^2 &= \frac{\pi}{a} \\
I &= \sqrt{\frac{\pi}{a}} \\
\int_{-\infty}^{\infty}{e^{-ax^2}}dx &= \sqrt{\frac{\pi}{a}} \\
\end{alignedat}
\end{gather*}
\end{theorem}

Since $e^{-ax^2}$ is an even function we also get the integral
\begin{equation}
\int_{0}^{\infty}{e^{-ax^2}}dx = \frac{\sqrt{\frac{\pi}{a}}}{2} = \sqrt{\frac{\pi}{4a}} 
\end{equation}

\section{Gaussian Type Integrals} 
Using $
\int_{-\infty}^{\infty}{e^{-ax^2}}dx = \sqrt{\frac{\pi}{a}}
$ we can take derivatives with respect to (w.r.t.) $a$
 
\begin{gather*}
\frac{\partial}{\partial a} \int_{-\infty}^{\infty}{e^{-ax^2}}dx = \frac{\partial}{\partial a} \sqrt{\frac{\pi}{a}}  \\
\int_{-\infty}^{\infty}{-x^2 e^{-ax^2}}dx = \sqrt{\pi} \frac{-1}{2} a^{-3/2} \\
\boxed{
\int_{-\infty}^{\infty}{x^2 e^{-ax^2}}dx = \frac{1}{2a}  \sqrt{\frac{\pi}{a}}
}\\
\end{gather*}
This process can be repeated to obtain the general identity

\begin{equation}
\boxed{
\int_{-\infty}^{\infty}{x^{2n} e^{-ax^2}}dx = \frac{\pi}{|\Gamma(\tfrac{1}{2} - n)|a^n \sqrt{a}}}
\end{equation}

\end{document}