\documentclass[a4paper]{article}

\usepackage[english]{babel}
\usepackage[utf8x]{inputenc}
\usepackage{amsmath}
\usepackage{graphicx}
\usepackage[colorinlistoftodos]{todonotes}
\usepackage{mathtools}

\title{Deriving the Quadratic equation}
\author{Emil Kerimov}
\date{\today}
\begin{document}
\maketitle

\section{The Quadratic Equation}

Given a quadratic polynomial $ax^2 + bx + c = 0$
The two solutions of $x$ that satisfy this equation are given by the quadratic equation
\begin{equation}
x = \frac{-b \pm \sqrt{b^2 - 4ac}}{2a}
\end{equation}

\section{Algebraic Proof}
The most straight-forward proof is given by a technique referred to as 'Completing the Square'.

\begin{gather*}
ax^2 + bx + c = 0\\
\shortintertext{Dividing both sides by $a$}
x^2 + \frac{b}{a}x + \frac{c}{a} = 0\\
\shortintertext{Adding and subtracting $\frac{b^2}{(2a)^2}$}
x^2 + \frac{b}{a}x + \frac{b^2}{(2a)^2} +  \frac{c}{a} - \frac{b^2}{(2a)^2} = 0\\
\shortintertext{Recognizing the 'square'}
(x+ \frac{b}{2a})^2 +  \frac{c}{a} - \frac{b^2}{(2a)^2} = 0\\
\shortintertext{Rearranging and solving}
\begin{alignedat}{2}
(x + \frac{b}{2a})^2 &= \frac{b^2}{4a^2}-  \frac{c}{a}  = \frac{b^2-4ac}{4a^2}\\
x + \frac{b}{2a} &=\pm \sqrt{ \frac{b^2 - 4ac}{4a^2}}\\
x  &= - \frac{b}{2a} \pm \sqrt{ \frac{b^2 - 4ac}{4a^2}}\\
x  &= \frac{-b \pm \sqrt{b^2 - 4ac}}{2a}\\
\end{alignedat}
\end{gather*}


\end{document}