\documentclass[a4paper]{article}

\usepackage[english]{babel}
\usepackage[utf8x]{inputenc}
\usepackage{amsmath}
\usepackage{graphicx}
\usepackage[colorinlistoftodos]{todonotes}
\usepackage{mathtools}

\title{One of Ramanujan Identity}
\author{Emil Kerimov}
\date{\today}
\begin{document}
\maketitle

\section{Ramanujan Identity} \label{sec:ramanujan-identity}

Prove that:

$$\alpha \sum\limits_{k=1}^{\infty} \frac{k}{e^{2\alpha k}-1}  + \beta \sum\limits_{k=1}^{\infty} \frac{k}{e^{2\beta k}-1} = \frac{\alpha + \beta}{24} - \frac{1}{4}$$

$$\alpha>0, \beta>0, \alpha \cdot \beta = \pi^2$$



$$\displaystyle f(t)=\begin{cases} 
\frac{|t|}{e^{2\alpha |t|}-1} & t\neq 0  \\ 
\frac{1}{2\alpha} & t=0 
\end{cases}$$


$$\displaystyle \hat{f}(s)=\int_{-\infty}^{\infty}f(t) e^{-i2\pi st}dt= \int_{-\infty}^{\infty}f(t)\cos(2\pi st) dt + i\int_{-\infty}^{\infty}f(t) \sin(2\pi st)dt = 2\int_{0}^{\infty}\frac{t\cos(2\pi st)}{e^{2\alpha t}-1}dt \mbox{ and } s\neq 0$$

$$\displaystyle \hat{f}(0)= 2\int_{0}^{\infty}\frac{t}{e^{2\alpha t}-1}dt = \frac{2}{(2\alpha)^{2}}\zeta(2) = \frac{\pi^2}{12\alpha^2} \mbox{ (Insert Reference) }$$

Notice both the function and it's Fourier Transform are even.

By Poisson Summation formula (Include Reference):

$$\displaystyle \hat{f}(0) + 2\sum_{m=1}^{\infty} \hat{f}(m)
={f}(0) + 2\sum_{n=1}^{\infty} {f}(n)
$$

Hence applying this:

$$\frac{1}{2\alpha} + 2\sum_{n=1}^{\infty} \frac{n}{e^{2\alpha n}-1}
=\frac{\pi^2}{12\alpha^2} + 4\sum_{m=1}^{\infty} \int_{0}^{\infty}\frac{t\cos(2\pi mt)}{e^{2\alpha t}-1}dt
$$

Examining $$\int_{0}^{\infty}\frac{t\cos(2\pi mt)}{e^{2\alpha t}-1}dt$$

By considering $$\int_{0}^{\infty}\frac{\sin(cx)}{e^{x}-1}dx 
=\int_{0}^{\infty}\frac{e^{-x}\sin(cx)}{1-e^{-x}}dx
= \int_{0}^{\infty}\sin{cx}\sum\limits_{k=1}^{\infty} e^{-kx}dx
$$


By the Dominant Convergence Theorem: (Include Reference)


$$\int_{0}^{\infty}\sin(cx)\sum\limits_{k=1}^{\infty} e^{-kx}dx
=\sum\limits_{k=1}^{\infty} \int_{0}^{\infty}\sin(cx)e^{-kx} dx
$$

By the LaPlace Transform of $\sin{at}$:

$$\int_{0}^{\infty}\sin(ct)e^{-sx} dt
=\frac{c}{c^2 + s^2} \mbox{  (Insert Reference)}
$$

$$
\sum\limits_{k=1}^{\infty} \int_{0}^{\infty}\sin(cx)e^{-kx} dx
=\sum\limits_{k=1}^{\infty} \frac{c}{c^2+k^2}
$$

By the Tangent Identity (Insert Reference)
$$\sum\limits_{n=-\infty}^{\infty} \frac{1}{\alpha^2+n^2}
=\frac{\pi}{\alpha}\coth(\pi \alpha)$$

Where $$\coth(x)=\frac{\cosh(x)}{\sinh(x)}=\frac{e^{x}+e^{-x}}{e^{x}-e^{-x}}
=\frac{e^{2x}+1}{e^{2x}-1}
$$

Hence:
$$\sum\limits_{n=-\infty}^{\infty} \frac{1}{\alpha^2+n^2}
=\frac{\pi}{\alpha}\cdot\frac{e^{2\pi \alpha}+1}{e^{2\pi \alpha}-1}
$$

Hence:
$$\sum\limits_{n=1}^{\infty} \frac{1}{\alpha^2+n^2}
=\frac{1}{2}\cdot(\frac{\pi}{\alpha}\cdot\frac{e^{2\pi \alpha}+1}{e^{2\pi \alpha}-1} - \frac{1}{\alpha^2})
$$

$$=> 
\sum\limits_{k=1}^{\infty} \frac{c}{c^2+k^2}
=\frac{\pi}{2}\cdot\frac{e^{2\pi c}+1}{e^{2\pi c}-1} - \frac{1}{2c}
$$

$$=>
\int_{0}^{\infty}\frac{\sin(cx)}{e^{x}-1}dx
=\frac{\pi}{2}\cdot\frac{e^{2\pi c}+1}{e^{2\pi c}-1} - \frac{1}{2c}
$$

Taking the derivative of both sides using Leibniz Rule

$$
\frac{d}{dc}\int_{0}^{\infty}\frac{\sin(cx)}{e^{x}-1}dx
=\int_{0}^{\infty}\frac{\partial}{\partial c}\frac{\sin(cx)}{e^{x}-1}dx
=\int_{0}^{\infty}\frac{x\cos(cx)}{e^{x}-1}dx
$$

$$=\frac{d}{dc}(\frac{\pi}{2}\cdot\frac{e^{2\pi c}+1}{e^{2\pi c}-1} - \frac{1}{2c})
= \frac{\pi}{2}\cdot\frac{2\pi e^{2\pi c}}{e^{2\pi c}-1} -\frac{\pi}{2}\cdot\frac{2\pi e^{4\pi c}+2\pi e^{2\pi c}}{(e^{2\pi c}-1)^2} + \frac{1}{2c^2}
= \frac{-2\pi^2e^{2\pi c}}{(e^{2\pi c}-1)^2} + \frac{1}{2c^2}
$$


Therefore making a change of variables $x=2\alpha t$
$$
\int_{0}^{\infty}\frac{x\cos(cx)}{e^{x}-1}dx
=\int_{0}^{\infty}\frac{2\alpha t\cos(2\alpha ct)}{e^{2\alpha t}-1}2\alpha dt
=(2\alpha)^2\int_{0}^{\infty}\frac{t\cos(2\alpha ct)}{e^{2\alpha t}-1}dt
=\frac{-2\pi^2e^{2\pi c}}{(e^{2\pi c}-1)^2} + \frac{1}{2c^2}
$$

Letting $c=\pi \cdot \frac{m}{\alpha}$ 

$$
(2\alpha)^2\int_{0}^{\infty}\frac{t\cos(2 \pi m \cdot t)}{e^{2\alpha t}-1}dt
=\frac{-2\pi^2e^{2\pi^2 \cdot \frac{m}{\alpha}}}{(e^{2\pi^2 \cdot \frac{m}{\alpha}}-1)^2} + \frac{1}{2\pi^2 \cdot \frac{m^2}{\alpha^2}}
=\frac{-2\pi^2e^{2\pi^2 \cdot \frac{m}{\alpha}}}{(e^{2\pi^2 \cdot \frac{m}{\alpha}}-1)^2} + \frac{\alpha^2}{2\pi^2 m^2}
$$

Plugging this result back into our original statement:

$$\frac{1}{2\alpha} + 2\sum_{n=1}^{\infty} \frac{n}{e^{2\alpha n}-1}
=\frac{\pi^2}{12\alpha^2} + \sum_{m=1}^{\infty} (\frac{-2\pi^2e^{2\pi^2 \cdot \frac{m}{\alpha}}}{\alpha^2(e^{2\pi^2 \cdot \frac{m}{\alpha}}-1)^2} + \frac{1}{2\pi^2 m^2})
=\frac{\pi^2}{12\alpha^2} + \sum_{m=1}^{\infty} \frac{-2\pi^2e^{2\pi^2 \cdot \frac{m}{\alpha}}}{\alpha^2(e^{2\pi^2 \cdot \frac{m}{\alpha}}-1)^2} + \frac{1}{2\pi^2}\zeta(2)
$$

$$
\frac{1}{2\alpha} + 2\sum_{n=1}^{\infty} \frac{n}{e^{2\alpha n}-1}
=\frac{\pi^2}{12\alpha^2} + \sum_{m=1}^{\infty} \frac{-2\pi^2e^{2\pi^2 \cdot \frac{m}{\alpha}}}{\alpha^2(e^{2\pi^2 \cdot \frac{m}{\alpha}}-1)^2} + \frac{1}{12}
$$

Let $\beta = \frac{\pi^2}{\alpha}$
$$=>
\frac{1}{2\alpha} + 2\sum_{n=1}^{\infty} \frac{n}{e^{2\alpha n}-1}
=\frac{\pi^2}{12\alpha^2}+ \frac{1}{12} -\frac{2\pi^2}{\alpha^2}\sum_{m=1}^{\infty} \frac{e^{2m\beta}}{(e^{2m\beta}-1)^2}
$$

Examining $\sum_{m=1}^{\infty} \frac{e^{2m\beta}}{(e^{2m\beta}-1)^2}$

$$
\sum_{n=1}^{\infty} \frac{n}{e^{2\beta n}-1}
=\sum_{n=1}^{\infty} \frac{ne^{-2\beta n}}{1-e^{-2\beta n}}
=\sum_{n=1}^{\infty} (n\sum_{m=1}^{\infty} e^{-2\beta \cdot n \cdot m})
$$

$$
\sum_{n=1}^{\infty} (n\sum_{m=1}^{\infty} e^{-2\beta \cdot n \cdot m})
=\sum_{n=1}^{\infty}\sum_{m=1}^{\infty} ne^{-2\beta \cdot n \cdot m}
=\sum_{m=1}^{\infty}\sum_{n=1}^{\infty} ne^{-2\beta \cdot n \cdot m}
$$

Insert Reference from Geometric Series Section

$$
\sum_{m=1}^{\infty}\frac{e^{-2\beta \cdot m}}{(1-e^{-2\beta \cdot m})^2}
=\sum_{m=1}^{\infty}\frac{e^{2\beta \cdot m}}{(e^{2\beta \cdot m}-1)^2}
=\sum_{n=1}^{\infty} \frac{n}{e^{2\beta n}-1}
$$

Hence combining this fact we obtain:

$$=>
\frac{1}{2\alpha} + 2\sum_{n=1}^{\infty} \frac{n}{e^{2\alpha n}-1}
=\frac{\pi^2}{12\alpha^2}+ \frac{1}{12} -\frac{2\pi^2}{\alpha^2}\sum_{n=1}^{\infty} \frac{n}{e^{2\beta n}-1}
$$

$$
\frac{1}{2\alpha} + 2\sum_{n=1}^{\infty} \frac{n}{e^{2\alpha n}-1}
=\frac{\beta}{12\alpha}+ \frac{1}{12} -\frac{2\beta}{\alpha}\sum_{n=1}^{\infty} \frac{n}{e^{2\beta n}-1}
$$

$$
\frac{1}{2} + 2\alpha \sum_{n=1}^{\infty} \frac{n}{e^{2\alpha n}-1}
=\frac{\beta}{12}+ \frac{\alpha}{12} -2\beta\sum_{n=1}^{\infty} \frac{n}{e^{2\beta n}-1}
$$

$$\boxed{
\alpha \sum_{n=1}^{\infty} \frac{n}{e^{2\alpha n}-1}+\beta\sum_{n=1}^{\infty} \frac{n}{e^{2\beta n}-1}
=\frac{\beta+\alpha}{24}- \frac{1}{4}
}
$$

Where $\alpha \cdot \beta = \pi^2$

The special case of $\alpha=\beta=\pi$:

$$
\boxed{
\sum_{n=1}^{\infty} \frac{n}{e^{2\pi n}-1}
=\frac{1}{24}- \frac{1}{8\pi}
}
$$

\end{document}